chore: update to v4.13.0

Regex/Data/Array/Basic.lean
@@ -2,25 +2,25 @@ namespace Array
 
 /-- get head element and array without head element -/
 def head? (a : Array α) : Option (α × Array α) :=
-  match a.data with
+  match a.toList with
   | [] => none
   | List.cons head tail => some (head, ⟨tail⟩)
 
 /-- get last element and array without last element -/
 def pop? (a : Array α) : Option (α × Array α) :=
-  if h : 0 < a.data.length
-  then some ((a.data.get ⟨a.data.length - 1, Nat.sub_lt h Nat.one_pos⟩), a.pop)
+  if h : 0 < a.toList.length
+  then some ((a.toList.get ⟨a.toList.length - 1, Nat.sub_lt h Nat.one_pos⟩), a.pop)
   else none
 
 /-- get last element of array -/
 def last? (a : Array α) : Option α :=
-  if h : 0 < a.data.length
-  then a.data.get ⟨a.data.length - 1, Nat.sub_lt h Nat.one_pos⟩
+  if h : 0 < a.toList.length
+  then a.toList.get ⟨a.toList.length - 1, Nat.sub_lt h Nat.one_pos⟩
   else none
 
 /-- unique array of sorted array -/
 def unique [BEq α] (intervals: Array α) : Array α :=
-  match intervals.data with
+  match intervals.toList with
   | [] => #[]
   | [r] => #[r]
   | head :: tail  =>
