Regex/Data/Array/Lemmas.lean
@@ -1,4 +1,3 @@
-import Batteries.Data.Nat.Lemmas
 import Init.Data.List.Lemmas
 import Init.Data.Array.Mem
 
@@ -11,7 +10,7 @@ theorem sizeOf_head?_of_mem [SizeOf α] {as : Array α} (h : Array.head? as = so
     : sizeOf a < sizeOf as := by
   unfold Array.head? at h
   split at h <;> simp_all
-  exact Array.sizeOf_lt_of_mem <| (Array.mem_def a as).mpr (by simp_all)
+  exact Array.sizeOf_lt_of_mem <| (@Array.mem_def α a as).mpr (by simp_all)
 
 theorem sizeOf_head?_of_tail [SizeOf α] {as : Array α} (h : Array.head? as = some (a, as'))
     : sizeOf as' < sizeOf as := by
@@ -34,7 +33,7 @@ theorem sizeOf_dropLast_non_empty [SizeOf α] (as : List α) (h : 0 < as.length)
   split at h <;> simp_all
   exact sizeOf_dropLast_cons _ _
 
-theorem sizeOf_pop_non_empty [SizeOf α] (as : Array α) (h : 0 < as.data.length)
+theorem sizeOf_pop_non_empty [SizeOf α] (as : Array α) (h : 0 < as.toList.length)
     : sizeOf as.pop < sizeOf as := by
   unfold Array.pop
   cases as with | _ as =>
@@ -71,38 +70,38 @@ theorem pop?_of_non_empty (arr : Array α) (h : 0 < arr.size)
   unfold Array.pop?
   split <;> simp_all
 
-theorem last?_eq_getLast (a : Array α) (h1: Array.last? a = some last) (h2 : a.data ≠ [])
-    : List.getLast a.data h2 = last := by
+theorem last?_eq_getLast (a : Array α) (h1: Array.last? a = some last) (h2 : a.toList ≠ [])
+    : List.getLast a.toList h2 = last := by
   unfold Array.last? at h1
   split at h1 <;> simp_all
   rw [← h1]
-  simp [List.getLast_eq_getElem a.data h2]
+  simp [List.getLast_eq_getElem a.toList h2]
 
 theorem lt_of_pop?_eq_last? {arr : Array α} (h : Array.pop? arr = some (last, arr'))
-    : 0 < arr.data.length := by
+    : 0 < arr.toList.length := by
   unfold Array.pop? at h
   split at h <;> simp_all
 
 theorem get_last_of_pop? {arr : Array α} (h1 : Array.pop? arr = some (last, arr'))
-  (h2 : arr.data.length - 1 < arr.data.length)
-    : List.get arr.data ⟨arr.data.length - 1, h2⟩ = last := by
+  (h2 : arr.toList.length - 1 < arr.toList.length)
+    : List.get arr.toList ⟨arr.toList.length - 1, h2⟩ = last := by
   unfold Array.pop? at h1
   split at h1 <;> try simp_all
 
 theorem concat_of_pop? {arr : Array α} (h : Array.pop? arr = some (last, arr'))
-    : arr.data = arr'.data ++ [last] := by
-  have hlt : 0 < arr.data.length := by simp_all[Array.lt_of_pop?_eq_last? h]
-  have hlt : arr.data.length - 1 < arr.data.length := Nat.pred_lt_of_lt hlt
-  have hlast : List.get arr.data ⟨arr.data.length - 1, hlt⟩ = last :=
+    : arr.toList = arr'.toList ++ [last] := by
+  have hlt : 0 < arr.toList.length := by simp_all[Array.lt_of_pop?_eq_last? h]
+  have hlt : arr.toList.length - 1 < arr.toList.length := Nat.pred_lt_of_lt hlt
+  have hlast : List.get arr.toList ⟨arr.toList.length - 1, hlt⟩ = last :=
      Array.get_last_of_pop? h hlt
   unfold Array.pop? at h
   split at h <;> simp_all
   have hr : Array.pop arr = arr' := h
-  have hr : (Array.pop arr).data = arr'.data := by simp_all
-  have hx : (Array.pop arr).data = List.dropLast arr.data := Array.pop_data arr
+  have hr : (Array.pop arr).toList = arr'.toList := by simp_all
+  have hx : (Array.pop arr).toList = List.dropLast arr.toList := Array.pop_toList arr
   rw [hx] at hr
-  have hy : List.dropLast (arr'.data ++ [last]) = arr'.data := by apply List.dropLast_concat
-  have hz : List.dropLast arr.data = List.dropLast (arr'.data ++ [last]) := by
+  have hy : List.dropLast (arr'.toList ++ [last]) = arr'.toList := by apply List.dropLast_concat
+  have hz : List.dropLast arr.toList = List.dropLast (arr'.toList ++ [last]) := by
     rw [← hy] at hr
     rw [hr]
   simp [List.eq_of_dropLast_eq_last_eq hz hlt (by simp_all)
